src/dvspec/dafny-block-dv/utils/block_common_functions.dfy
@@ -32,21 +32,13 @@ module BlockCommonFunctions{
         forall i, j | 0 <= i < |s| && 0 <= j < |s| :: s[i] == s[j] ==> i == j
     }
 
-    predicate method {:extern} verify_bls_siganture<T>(
-        data: T,
-        signature: BLSSignature,
-        pubkey: BLSPubkey
-    )
-
     function method {:extern} hash_tree_root<T>(data: T): Root 
 
     function getMessagesFromMessagesWithRecipient<M>(mswr: set<MessaageWithRecipient<M>>): set<M>
     {
         set mwr | mwr in mswr :: mwr.message
     }
-   
-
-    /*
+       
     function addReceipientToMessages<M>(sm: set<M>, r: BLSPubkey): set<MessaageWithRecipient<M>>
     {
         set m | m in sm :: MessaageWithRecipient(
@@ -58,8 +50,7 @@ module BlockCommonFunctions{
     function addRecepientsToMessage<M>(m: M, receipients: set<BLSPubkey>): set<MessaageWithRecipient<M>>
     {
         set r | r in receipients :: MessaageWithRecipient(message := m, receipient := r)
-    }
-    */
+    }    
 
     function wrapMessagesWithRecipient<M>(sm: set<M>, r: BLSPubkey): set<MessaageWithRecipient<M>>
     {
@@ -110,4 +101,106 @@ module BlockCommonFunctions{
         var e: int :| e in s && forall e' | e' in s :: e' >= e;
         e        
     }
+
+    
+
+    // consensus_is_valid_block is for line 174
+    /*
+    method consensus_is_valid_block(
+        block_slashing_db: set<SlashingDBBlock>,
+        block: BeaconBlock,
+        proposer_duty: ProposerDuty,
+        complete_signed_randao_reveal: BLSSignature)
+    returns (b: bool) 
+    {
+        // TODO: Add correct block.proposer_index check
+        var slashable: bool;
+        slashable := is_slashable_block(block_slashing_db, block, proposer_duty.pubkey);
+        b := block.slot == proposer_duty.slot &&            
+             block.body.randao_reveal == complete_signed_randao_reveal &&
+             !slashable;                 
+    }
+    */
+    predicate method consensus_is_valid_block(
+        block_slashing_db: set<SlashingDBBlock>,
+        block: BeaconBlock,
+        proposer_duty: ProposerDuty,
+        complete_signed_randao_reveal: BLSSignature)
+    
+    {
+        // TODO: Add correct block.proposer_index check        
+        && block.slot == proposer_duty.slot 
+        && block.body.randao_reveal == complete_signed_randao_reveal
+        && !is_slashable_block(block_slashing_db, block, proposer_duty.pubkey)
+    }
+
+    // 
+    function method get_slashing_slots(slashing_db: BlockSlashingDB): (slots_in_db: set<int>)    
+    requires slashing_db != {}
+    ensures slots_in_db != {}    
+    {
+        var slots_in_db := set block | block in slashing_db :: block.slot;
+        assert var e :| e in slashing_db; e.slot in slots_in_db;
+        slots_in_db
+    }
+
+    // NOTE: Left this method here just in case, but it is currently not being used anywhere.
+    // function method get_slashing_blocks_with_slot(
+    //     slashing_db: BlockSlashingDB, 
+    //     slot: Slot
+    // ): (slashing_blocks: set<SlashingDBBlock>)    
+    // requires slashing_db != {}        
+    // {
+    //     var slashing_blocks := set block | block in slashing_db && block.slot == slot :: block;            
+    //     slashing_blocks
+    // }
+
+    // is_slashable_block is for line 153 in helpers.py
+    predicate is_slashable_block(
+        block_slashing_db: set<SlashingDBBlock>,
+        block: BeaconBlock, 
+        pubkey: BLSPubkey
+    ) 
+    {
+        if block_slashing_db != {} then
+        
+            var slots := get_slashing_slots(block_slashing_db);
+            var min_slot := get_min(slots);
+
+            if block.slot < min_slot then
+                true
+            else 
+                if exists db_block :: db_block in block_slashing_db && 
+                                      block.slot == db_block.slot &&
+                                      hash_tree_root(block) != db_block.signing_root
+                then 
+                    true
+                else
+                    false
+        else 
+            false
+    } by method
+    {            
+        
+        if block_slashing_db != {}
+        {
+            var slots := get_slashing_slots(block_slashing_db);
+            var min_slot := get_min(slots);
+
+            if block.slot < min_slot 
+            {
+                return true;
+            }
+            
+            if exists db_block :: db_block in block_slashing_db && 
+                                    block.slot == db_block.slot &&
+                                    hash_tree_root(block) != db_block.signing_root
+            {
+                return true;
+            }
+        }
+        
+        return false;            
+    }     
+
 }
